Getting closer..

lib/run.rb
@@ -2,10 +2,10 @@
 
 def one_test(c_src)
   system("clang -I/usr/local/include/smack #{c_src} -c -emit-llvm -o a.o")
-  system("smack a.o")
+  system("smack a.o -mem-mod-dbg")
   system("rm a.o")
   system("cat #{File.dirname(__FILE__)}/monitor.bpl >> a.bpl")
-  system("violin.rb a.bpl --verifier boogie_fi -l 3 -d 3")
+  system("violin.rb a.bpl --verifier boogie_si -l 3 -d 3 -k -v -g")
   system("rm a.bpl")
 end
 
