lib/monitor.bpl
@@ -1,10 +1,4 @@
 /******************************************************************************/
-/******************************************************************************/
-/**   DEMO  OF  USING  BOOGIE  FOR  OBSERVATIONAL REFINEMENT  VERIFICATION   **/
-/******************************************************************************/
-/******************************************************************************/
-
-/******************************************************************************/
 /*         GENERIC           CODE          FOR           OPERATIONS           */
 /******************************************************************************/
 
@@ -45,7 +39,7 @@ modifies N;
 {
   o := N;
   assume (forall oo: op :: completed(oo,C) ==> bef(oo,o));
-  assume (forall oo: op :: active(oo,N,C) ==> !(o <: oo) && !(oo <: o));
+  assume (forall oo: op :: active(oo,N,C) ==> !bef(o,oo) && !bef(oo,o));
   N := N + 1;
 }
 
@@ -68,101 +62,108 @@ function match(o1: op, o2: op) returns (bool) {
   m(o1) == add && m(o2) == remove && v(o1) == v(o2) 
 }
 
-function no_thinair(N: int, C: [op] bool, A: [int] bool) returns (bool) {
+function {:spec} no_thinair(N: int, C: [op] bool, A: [int] bool) returns (bool) {
   (forall o: op :: completed(o,C) && m(o) == remove ==> 
     A[v(o)] || v(o) == empty
   )
 }
 
-function unique_removes(N: int, C: [op] bool) returns (bool) {
+function {:spec} unique_removes(N: int, C: [op] bool) returns (bool) {
   (forall o1, o2: op :: completed(o1,C) && completed(o2,C) && o1 != o2 ==>  
     m(o1) != m(o2) || v(o1) != v(o2) || v(o1) == empty || v(o2) == empty
   )
 }
 
-function no_false_empty(N: int, C: [op] bool, E: [op] bool) returns (bool) {
-  (forall o: op :: completed(o,C) && m(o) == remove && v(o) == empty ==> E[o])
+function {:spec} no_false_empty(N: int, C: [op] bool, W: [op] bool) returns (bool) {
+  (forall o: op :: completed(o,C) && m(o) == remove && v(o) == empty ==> W[o])
 }
 
-function {:spec} bag_spec(N: int, C: [op] bool, A: [val] bool, E: [op] bool) 
+function {:spec} bag_spec(N: int, C: [op] bool, A: [val] bool, W: [op] bool) 
 returns (bool) {
-  no_thinair(N,C,A) && unique_removes(N,C) && no_false_empty(N,C,E)
+  no_thinair(N,C,A) && unique_removes(N,C) && no_false_empty(N,C,W)
 }
 
-function stack_order(N: int, C: [op] bool) returns (bool) {
+function {:spec} stack_order(N: int, C: [op] bool) returns (bool) {
   (forall o1, o2, o1', o2': op ::
     started(o1,N) && started(o2,N) && completed(o1',C) && completed(o2',C)
     && uniq4(o1,o2,o1',o2') 
     && match(o1,o1') && match(o2,o2')
-    && o1' <: o2' ==> bef?(o2,o1) || (bef?(o1,o2) && bef?(o1',o2))
+    && bef(o1',o2') ==> bef?(o2,o1) || (bef?(o1,o2) && bef?(o1',o2))
   )
 }
 
-function queue_order(N: int, C: [op] bool) returns (bool) {
+function {:spec} queue_order(N: int, C: [op] bool) returns (bool) {
   (forall o1, o2, o1', o2': op :: 
     started(o1,N) && started(o2,N) && completed(o1',C) && completed(o2',C)
     && uniq4(o1,o2,o1',o2')
     && match(o1,o1') && match (o2,o2')
-    && o1' <: o2' ==> bef?(o1,o2)
+    && bef(o1',o2') ==> bef?(o1,o2)
   )
 }
 
-function {:spec} stack_spec(N: int, C: [op] bool, A: [val] bool, E: [op] bool)
+function {:spec} stack_spec(N: int, C: [op] bool, A: [val] bool, W: [op] bool)
 returns (bool) {
-  bag_spec(N,C,A,E) && stack_order(N,C)
+  bag_spec(N,C,A,W) && stack_order(N,C)
 }
 
-function {:spec} queue_spec(N: int, C: [op] bool, A: [val] bool, E: [op] bool)
+function {:spec} queue_spec(N: int, C: [op] bool, A: [val] bool, W: [op] bool)
 returns (bool) {
-  bag_spec(N,C,A,E) && queue_order(N,C)
+  bag_spec(N,C,A,W) && queue_order(N,C)
 }
 
-var A: [val] bool;
-var low, high: int;
-// invariant (low <= high)
-var E: [op] bool;
+var A, R: [val] bool;
+var W: [op] bool;
+
+function sees_empty(A: [val] bool, R: [val] bool) returns (bool) {
+  (forall v: val :: A[v] ==> R[v])
+}
+
+procedure see_empty();
+modifies W;
+ensures sees_empty(A,R) ==> (forall o: op :: active(o,N,C) ==> W[o]);
+ensures sees_empty(A,R) ==> (forall o: op :: !active(o,N,C) ==> W[o] == old(W[o]));
 
 procedure {:init} init()
 modifies N, C;
-modifies A, low, high;
 {
   call op.init();
   assume (forall v: val :: !A[v]);
-  assume (forall o: op :: !E[o]);
-  low := 0;
-  high := 0;
+  assume (forall v: val :: !R[v]);
+  assume (forall o: op :: !W[o]);
 }
 
 procedure add.start(v: val) returns (o: op)
 modifies N;
-modifies A, high;
 {
+  call boogie_si_record_int(v);
   call o := op.start();
   assume m(o) == add;
   assume v(o) == v;
-  A[v] := true;
-  high := high + 1;
   return;
 }
 
 procedure add.finish(o: op)
 modifies C;
-modifies low;
+modifies A;
 {
   call op.finish(o);
-  low := low + 1;
+  A[v(o)] := true;
 }
 
 procedure remove.start() returns (o: op)
 modifies N;
-modifies low, E;
+modifies R, W;
 {
   call o := op.start();
+  call boogie_si_record_int(o);
   assume m(o) == remove;
-  E[o] := (low <= 0);
-  if (v(o) != empty) {
-    low := low - 1;
-    if (low == 0) {
+  if (v(o) == empty) {
+    W[o] := sees_empty(A,R);
+    call boogie_si_record_bool(W[o]);
+    
+  } else {
+    R[v(o)] := true;
+    if (sees_empty(A,R)) {
       call see_empty();
     }
   }
@@ -171,18 +172,9 @@ modifies low, E;
 
 procedure remove.finish(o: op, v: val)
 modifies C;
-modifies high, E;
 {
+  call boogie_si_record_int(v);
   assume v(o) == v;
   call op.finish(o);
-  if (v(o) != empty) {
-    high := high - 1;
-  }
   return;
 }
-
-procedure see_empty();
-modifies E;
-ensures low == 0 ==> (forall o: op :: active(o,N,C) ==> E[o]);
-ensures low == 0 ==> 
-  (forall o: op :: !active(o,N,C) ==> E[o] == old(E[o]));
